src/example/AuthExclAnysRA.v
@@ -1,0 +1,96 @@
+From sflib Require Import sflib.
+From Fairness Require Import Any PCM IProp IPM IPropAux.
+
+
+Section AEAPROP.
+
+  Definition AuthExclAnysRA : URA.t := (nat ==> (Auth.t (Excl.t Any.t)))%ra.
+
+  Context `{Σ : GRA.t}.
+  (* Map from nat to Auth Excl Any. *)
+  Context {AuthExclAnys : @GRA.inG AuthExclAnysRA Σ}.
+
+  Definition AuExAnyB_ra (r : nat) {T : Type} (t : T) : AuthExclAnysRA :=
+    ((maps_to_res r (Auth.black ((Some (t ↑)) : Excl.t Any.t))) : AuthExclAnysRA).
+  Definition AuExAnyW_ra (r : nat) {T : Type} (t : T) : AuthExclAnysRA :=
+    ((maps_to_res r (Auth.white ((Some (t ↑)) : Excl.t Any.t))) : AuthExclAnysRA).
+
+  Definition AuExAnyB (r : nat) {T : Type} (t : T) : iProp := OwnM (AuExAnyB_ra r t).
+  Definition AuExAnyW (r : nat) {T : Type} (t : T) : iProp := OwnM (AuExAnyW_ra r t).
+
+  Definition AuExAny : iProp :=
+    (∃ (U : nat), OwnM ((fun k => if (lt_dec k U)
+                             then ε
+                             else (Auth.black (Some (tt ↑) : Excl.t Any.t) ⋅ Auth.white (Some (tt ↑) : Excl.t Any.t)))
+                       : AuthExclAnysRA)).
+
+  (** Properties. *)
+
+  Lemma auexa_b_w_eq r T (tb tw : T) :
+    ⊢ AuExAnyB r tb -∗ AuExAnyW r tw -∗ ⌜tb = tw⌝.
+  Proof.
+    iIntros "B W". iCombine "B W" as "BW". iPoseProof (OwnM_valid with "BW") as "%WF".
+    iPureIntro. unfold AuExAnyB_ra, AuExAnyW_ra in WF. setoid_rewrite maps_to_res_add in WF.
+    unfold maps_to_res in WF. ur in WF. specialize (WF r). des_ifs. rewrite URA.unit_idl in WF.
+    ur in WF. des. unfold URA.extends in WF. des. ur in WF. des_ifs.
+    apply Any.upcast_inj in H0. des. rewrite EQ0. auto.
+  Qed.
+
+  Lemma auexa_b_b_false r T (t1 t2 : T) :
+    ⊢ AuExAnyB r t1 -∗ AuExAnyB r t2 -∗ False.
+  Proof.
+    iIntros "A B". iCombine "A B" as "C". iPoseProof (OwnM_valid with "C") as "%WF".
+    iPureIntro. unfold AuExAnyB_ra, AuExAnyW_ra in WF. setoid_rewrite maps_to_res_add in WF.
+    unfold maps_to_res in WF. ur in WF. specialize (WF r). des_ifs. ur in WF. auto.
+  Qed.
+
+  Lemma auexa_w_w_false r T (t1 t2 : T) :
+    ⊢ AuExAnyW r t1 -∗ AuExAnyW r t2 -∗ False.
+  Proof.
+    iIntros "A B". iCombine "A B" as "C". iPoseProof (OwnM_valid with "C") as "%WF".
+    iPureIntro. unfold AuExAnyB_ra, AuExAnyW_ra in WF. setoid_rewrite maps_to_res_add in WF.
+    unfold maps_to_res in WF. ur in WF. specialize (WF r). des_ifs. ur in WF. ur in WF. auto.
+  Qed.
+
+  Lemma auexa_b_w_update r T (t1 t2 : T) S (s : S) :
+    ⊢ AuExAnyB r t1 -∗ AuExAnyW r t2 ==∗ (AuExAnyB r s ∗ AuExAnyW r s).
+  Proof.
+    iIntros "B W".
+    assert (URA.updatable (AuExAnyB_ra r t1 ⋅ AuExAnyW_ra r t2)
+                          (AuExAnyB_ra r s ⋅ AuExAnyW_ra r s)).
+    { unfold AuExAnyB_ra, AuExAnyW_ra. setoid_rewrite maps_to_res_add. apply maps_to_updatable, Auth.auth_update.
+      ii. des. split.
+      - ur. ss.
+      - ur in FRAME. ur. des_ifs.
+    }
+    iCombine "B W" as "BW". iMod (OwnM_Upd with "BW") as "BW". eauto.
+    iDestruct "BW" as "[B W]". iModIntro. iFrame.
+  Qed.
+
+  Lemma auexa_alloc T (t : T) :
+    ⊢ AuExAny -∗ |==> (AuExAny ∗ ∃ r, AuExAnyB r t ∗ AuExAnyW r t).
+  Proof.
+    iIntros "[%U A]".
+    assert (URA.updatable
+              ((λ k : nat, if lt_dec k U
+                         then ε
+                         else(Auth.black (Some (tt ↑) : Excl.t Any.t) ⋅ Auth.white (Some (tt ↑) : Excl.t Any.t))) : AuthExclAnysRA)
+              (((λ k : nat, if lt_dec k (S U)
+                          then ε
+                          else(Auth.black (Some (tt ↑) : Excl.t Any.t) ⋅ Auth.white (Some (tt ↑) : Excl.t Any.t))) : AuthExclAnysRA)
+                 ⋅
+                 (AuExAnyB_ra U tt ⋅ AuExAnyW_ra U tt))).
+    { unfold AuExAnyB_ra, AuExAnyW_ra. setoid_rewrite maps_to_res_add. unfold maps_to_res. setoid_rewrite unfold_pointwise_add.
+      apply pointwise_updatable. i. des_ifs; try lia.
+      - rewrite URA.unit_id. reflexivity.
+      - rewrite URA.unit_idl. reflexivity.
+      - rewrite URA.unit_id. reflexivity.
+    }
+    iMod (OwnM_Upd with "A") as "[A [B W]]". eauto.
+    iMod (auexa_b_w_update with "B W") as "BW".
+    iModIntro. iSplitL "A".
+    - iExists (S U). iFrame.
+    - iExists U. iFrame.
+  Qed.
+
+End AEAPROP.
